src/SchedSim.v
@@ -29,10 +29,9 @@ Tactic Notation "repl" constr(e) "with" constr(e') "at" ne_integer_list(n) "by" 
 Ltac destruct_itree itr :=
   let E := fresh "E" in
   destruct (observe itr) eqn: E;
-  let H := fresh "H" in
-  pose proof (H := itree_eta_ itr);
-  rewrite E in H;
-  clear E;
+  symmetry in E;
+  apply simpobs in E;
+  apply bisim_is_eq in E;
   subst itr.
 
 Section SIM.
@@ -50,6 +49,18 @@ Section SIM.
   Let thread R := thread _Ident (sE State) R.
   Import Th.
 
+  Lemma Empty_nil s : IdSet.Empty s -> IdSet.elements s = [].
+  Proof.
+    i. destruct s as [s OK]; ss. destruct s; ss.
+    exfalso. eapply H. econs. ss.
+  Qed.
+
+  Lemma Empty_nil_neg s : ~ IdSet.Empty s -> IdSet.elements s <> [].
+  Proof.
+    destruct s as [s SORTED]; ss.
+    ii. subst. eapply H. ii. eapply InA_nil; eauto.
+  Qed.
+
   Lemma In_MapsTo A k e (m : Th.t A) : List.In (k, e) (elements m) -> MapsTo k e m.
   Proof.
     unfold MapsTo, Raw.PX.MapsTo, elements, Raw.elements.
@@ -66,6 +77,50 @@ Section SIM.
     induction l; ss. destruct H.
     - eexists. eapply InA_cons_hd. subst. ss.
     - eapply IHl in H. destruct H. eexists. eapply InA_cons_tl. eauto.
+  Qed.
+
+  Lemma IdSet_Permutation_remove x s l :
+    Permutation (IdSet.elements s) (x :: l) -> Permutation (IdSet.elements (IdSet.remove x s)) l.
+  Proof.
+    destruct s as [s SORTED]. ss.
+    revert l. induction s; i.
+    - eapply Permutation_length in H. ss.
+    - assert (List.In a (x :: l)) by (rewrite <- H; econs; ss).
+      destruct H0.
+      + subst. eapply Permutation_cons_inv in H. ss.
+        Raw.MX.elim_comp_eq a a. ss.
+      + eapply Add_inv in H0. des. eapply Permutation_Add in H0.
+        rewrite <- H0 in *. clear l H0.
+        rewrite perm_swap in H. eapply Permutation_cons_inv in H.
+        assert (List.In x s).
+        { eapply Permutation_in.
+          - symmetry. eapply H.
+          - econs; ss.
+        }
+        eapply IdSet.MSet.Raw.isok_iff in SORTED.
+        epose proof (Sorted_extends _ SORTED).
+        eapply Forall_forall in H1; eauto.
+        ss. Raw.MX.elim_comp_gt x a.
+        econs. eapply IHs; eauto.
+        eapply IdSet.MSet.Raw.isok_iff.
+        inv SORTED; ss.
+    Unshelve. compute. lia.
+  Qed.
+
+  Lemma IdSet_Permutation_add x s l :
+    ~ IdSet.In x s -> Permutation (IdSet.elements s) l -> Permutation (IdSet.elements (IdSet.add x s)) (x :: l).
+  Proof.
+    destruct s as [s SORTED]. ss. revert l. induction s; intros l H1 H2.
+    - rewrite <- H2. ss.
+    - ss. assert (x = a \/ x < a \/ x > a) by lia. des.
+      + exfalso. eapply H1. econs. ss.
+      + Raw.MX.elim_comp_lt x a. econs. ss.
+      + Raw.MX.elim_comp_gt x a. rewrite <- H2. rewrite perm_swap. econs.
+        eapply IHs; eauto.
+        unfold IdSet.In, IdSet.MSet.In in *. ss.
+        intro. eapply H1. econs 2. eapply H0.
+        Unshelve. clear H1. eapply IdSet.MSet.Raw.isok_iff in SORTED. inv SORTED.
+        eapply IdSet.MSet.Raw.isok_iff. ss.
   Qed.
 
   Lemma Permutation_remove A k e (m : Th.t A) l :
@@ -113,6 +168,12 @@ Section SIM.
         destruct H0. eexists. right. eauto.
   Qed.
 
+  Lemma InA_In A x (l : list A) : InA (@eq A) x l -> List.In x l.
+  Proof. i. induction H.
+         - left; eauto.
+         - right; eauto.
+  Qed.
+    
   Lemma setoid_in_in A k (e : A) l :
     SetoidList.InA (@eq_key_elt A) (k, e) l -> List.In (k, e) l.
   Proof.
@@ -134,293 +195,270 @@ Section SIM.
   Lemma nth_error_Some' A (l : list A) x i : nth_error l i = Some x -> i < List.length l.
   Proof. i. eapply nth_error_Some. intro. rewrite H in H0; ss. Qed.
 
-  Theorem sched_sim
-    p_src p_tgt
-    st ths_src ths_tgt tid (itr : thread R)
-    (THREADS : Permutation (elements ths_src) ths_tgt)
-    (TID : forall itr0, ~ List.In (tid, itr0) ths_tgt)
-    : gsim nat_wf nat_wf eq p_src p_tgt (interp_all st ths_src tid itr) (interp_all_fifo st ths_tgt tid itr).
+  Theorem ssim_nondet_fifo
+    p_src p_tgt tid ths_src ths_tgt
+    (THREADS : Permutation (IdSet.elements ths_src) ths_tgt)
+    (TID : ~ IdSet.In tid ths_src)
+    : forall m_tgt, exists m_src, @ssim nat_wf nat_wf R R R eq p_src m_src p_tgt m_tgt
+                          (schedule_nondet R (tid, ths_src))
+                          (schedule_fifo R (tid, ths_tgt)).
   Proof.
-    unfold interp_all, interp_all_fifo, gsim. intro m_tgt.
+    i.
 
-    (* Choose m_src and invariants about it *)
-    remember (fun (i : (sum_tid _Ident).(id)) =>
-                match i with
-                | inl x => List.length ths_tgt + 1
-                | inr x => m_tgt (inr x)
-                end) as m_src.
-    assert (M_SRC0 : m_src (inl tid) > List.length ths_tgt) by (subst; lia).
-    assert (M_SRC1 : forall i tid t, nth_error ths_tgt i = Some (tid, t) -> m_src (inl tid) > i).
+    remember (fun (i : thread_id.(id)) => List.length ths_tgt + 1) as m_src.
+    assert (M_SRC0 : m_src tid > List.length ths_tgt) by (subst; lia).
+    assert (M_SRC1 : forall i tid, nth_error ths_tgt i = Some tid -> m_src tid > i).
     { subst. i. eapply nth_error_Some' in H. lia. }
-    assert (M_SRC2 : (forall i, m_src (inr i) = m_tgt (inr i))) by (subst; eauto).
     clear Heqm_src.
     exists m_src.
 
-    (* coinduction - outer loop *)
-    revert p_src p_tgt st ths_src ths_tgt tid itr m_tgt m_src THREADS TID M_SRC0 M_SRC1 M_SRC2.
-    pcofix CIH1. i.
+    revert p_src p_tgt m_src m_tgt tid ths_src ths_tgt THREADS TID M_SRC0 M_SRC1.
+    pcofix CIH. i.
 
-    rewrite unfold_interp_sched_nondet.
-    rewrite unfold_interp_fifosched.
-    rewrite 2 interp_state_bind.
-    rewrite unfold_interp_thread.
-    rewrite interp_state_aux_map_event.
-    match goal with
-    | [ |- paco9 _ _ _ _ _ _ _ _ _ (ITree.bind (map_event _ ?itr) ?ktr) _ ] => remember itr as itr0
-    end.
-    clear Heqitr0 itr st.
-
-    (* coinduction - inner loop *)
-    revert p_src p_tgt m_src m_tgt itr0 M_SRC0 M_SRC1 M_SRC2.
-    pcofix CIH2. i.
-
-    destruct_itree itr0; cycle 1.
-    - (* Tau *)
-      rewrite map_event_tau. grind. pfold; do 3 econs; eauto.
-    - (* Vis *)
-      rewrite map_event_vis. grind.
-      destruct e.
-      + pfold. rewrite <- 2 bind_trigger.
-        eapply sim_chooseR. intros.
-        eapply sim_chooseL. exists x.
-        econs; eauto.
-      + pfold. rewrite <- 2 bind_trigger.
-        eapply sim_fairR. intros.
-        eapply sim_fairL.
-        exists (fun i => match i with
-                 | inl x => m_src (inl x)
-                 | inr x => m_tgt0 (inr x)
-                 end).
-        splits.
-        * unfold fair_update. i.
-          destruct i; ss.
-          -- left. eauto.
-          -- rewrite M_SRC2.
-             unfold fair_update in FAIR.
-             specialize FAIR with (inr i).
-             ss.
-        * econs; eauto.
-      + ss. pfold. econs. intros. subst. right. eapply CIH2; eauto.
-      + ss. pfold. rewrite <- 2 bind_trigger. eapply sim_ub.
-    - (* Ret *)
-      clear CIH2. destruct r0 as [st r0]. rewrite map_event_ret. grind.
-      destruct r0 as [itr_yield | r0].
-      + (* Yield *)
-        rewrite pick_thread_nondet_yield.
-        rewrite pick_thread_fifo_yield.
-        rewrite bind_vis.
-        rewrite interp_state_vis.
-        rewrite <- bind_trigger.
-        match goal with
-        | [ |- paco9 _ _ _ _ _ _ _ _ _ _ (interp_state (_, _ <- match ?x with
-                                                              | [] => _
-                                                              | t' :: ts' => _
-                                                              end;;
-                                                          _))] => destruct x as [|[tid' itr'] ths_tgt'] eqn: E_ths_tgt
-        end.
-        { eapply app_eq_nil in E_ths_tgt. des. ss. }
-        rewrite bind_ret_l.
-        rewrite interp_state_tau.
-        pfold. do 2 econs. exists tid'. econs.
-        unfold th_pop.
-        replace (find tid' (add tid itr_yield ths_src)) with (Some itr').
-        2: {
-          symmetry. eapply find_1.
-          destruct ths_tgt.
-          - ss. inversion E_ths_tgt; subst.
-            eapply add_1; eauto.
-          - destruct p.
-            inversion E_ths_tgt; subst.
-            assert (tid' <> tid).
-            { pose proof (TID itr').
-              intro H1. eapply H. left. subst. ss.
-            }
-            eapply add_2; eauto.
-            eapply In_MapsTo.
-            rewrite THREADS.
-            left. ss.
+    rewrite unfold_schedule_nondet.
+    rewrite unfold_schedule_fifo.
+    rewrite ! bind_trigger.
+    pfold. econs. intros [].
+    - left.
+      destruct (IdSet.is_empty ths_src) eqn: H.
+      + eapply IdSet.is_empty_2 in H.
+        eapply Empty_nil in H.
+        rewrite H in THREADS.
+        eapply Permutation_nil in THREADS.
+        subst ths_tgt.
+        pfold. econs; ss.
+      + assert (~ IdSet.Empty ths_src).
+        { ii. eapply IdSet.is_empty_1 in H0. rewrite H in H0; ss. }
+        clear H. eapply Empty_nil_neg in H0.
+        destruct ths_tgt as [| tid' ths_tgt' ].
+        { symmetry in THREADS. eapply Permutation_nil in THREADS. ss. }
+        pfold. eapply ssim_chooseL. exists tid'. unfold id_pop.
+        replace (IdSet.mem tid' ths_src) with true; cycle 1.
+        { symmetry. eapply IdSet.mem_1. eapply In_InA; eauto.
+          rewrite THREADS. econs; ss.
         }
-        rewrite bind_vis.
-        rewrite interp_state_vis.
-        rewrite <- bind_trigger.
-        eapply sim_fairL.
-        exists (fun i => match i with
-                 | inl x => if Nat.eqb x tid'
-                           then List.length ths_tgt' + 1
-                           else m_src (inl x) - 1
-                 | inr x => m_src (inr x)
-                 end).
-        splits.
-        { unfold fair_update. i. destruct i; ss.
-          - unfold tids_fmap.
-            des_if; eauto.
-            replace (Nat.eqb i tid') with false
-              by (symmetry; eapply Nat.eqb_neq; eauto).
-            des_if.
-            + eapply In_th_proj1 in i0.
-              destruct i0.
-              eapply remove_3 in H.
-              assert (i = tid \/ i <> tid) by lia.
-              destruct H0.
-              * subst i. unfold key in *. lia.
-              * eapply add_3 in H; eauto.
-                eapply elements_1 in H.
-                unfold elements, Raw.elements in H.
-                eapply setoid_in_in in H.
-                eapply Permutation_in in H.
-                2: eapply THREADS.
-                eapply In_nth_error in H.
-                destruct H as [j H].
-                enough (m_src (inl i) > j) by lia.
-                eapply M_SRC1.
-                eauto.
-            + unfold le. ss. lia.
-          - left. ss.
+        rewrite bind_trigger.
+        eapply ssim_fairL.
+        remember (fun i => if Nat.eqb i tid'
+                        then List.length ths_tgt' + 1
+                        else m_src i - 1) as m_src'.
+        exists m_src'. splits.
+        { ii. unfold tids_fmap. des_if; ss. subst.
+          replace (i =? tid')%nat with false by (symmetry; eapply Nat.eqb_neq; eauto).
+          des_if.
+          - assert (List.In i (IdSet.elements ths_src)).
+            { eapply InA_In. eapply IdSet.remove_3. eapply In_InA; eauto. eapply i0. }
+            rewrite THREADS in H.
+            eapply In_nth_error in H. destruct H as [i' H].
+            enough (m_src i > i') by lia.
+            eapply M_SRC1; eauto.
+          - unfold le; ss. lia.
         }
-        rewrite bind_ret_l.
-        rewrite interp_state_tau.
-        do 3 econs; eauto. right. unfold key in *; ss. eapply CIH1.
-        * eapply Permutation_remove.
-          transitivity ([(tid, itr_yield)] ++ ths_tgt).
-          { eapply Permutation_add; ss. intro H.
-            unfold In, Raw.PX.In, Raw.PX.MapsTo in H. destruct H.
-            eapply setoid_in_in in H. rewrite THREADS in H.
-            eapply TID; eauto.
-          }
-          transitivity (ths_tgt ++ [(tid, itr_yield)]).
-          { eapply Permutation_app_comm. }
-          rewrite E_ths_tgt. ss.
-        * intros itr0 H.
-          pose proof (elements_3w ths_src).
-          eapply (Permutation_NoDupA _ _ _ THREADS) in H0.
-          inversion H0; subst; inversion E_ths_tgt; subst.
-          -- inversion H.
-          -- eapply H1.
-             eapply SetoidList.InA_eqA; eauto.
-             instantiate (1 := (tid', itr0)); ss.
-             eapply SetoidList.In_InA; eauto.
-             eapply in_app_or in H. 
-             destruct H; eauto. exfalso.
-             assert (tid = tid') by (destruct H; ss; inversion H; ss).
-             eapply TID. left. subst. ss.
-        * replace (tid' =? tid')%nat with true by (symmetry; eapply Nat.eqb_refl). lia.
-        * i. des_if.
+        do 3 econs; eauto. right. eapply CIH.
+        * eapply IdSet_Permutation_remove. eapply THREADS.
+        * eapply IdSet.remove_1; ss.
+        * subst. replace (tid' =? tid')%nat with true by (symmetry; eapply Nat.eqb_refl). lia.
+        * subst. i. des_if.
           -- eapply nth_error_Some' in H. lia.
-          -- enough (m_src (inl tid0) > 1 + i) by lia.
-             assert (nth_error (ths_tgt ++ [(tid, itr_yield)]) (1 + i) = Some (tid0, t0))
-               by (rewrite E_ths_tgt; ss).
-             assert (1 + i < List.length ths_tgt \/ 1 + i >= List.length ths_tgt) by lia.
-             destruct H1.
-             ++ rewrite nth_error_app1 in H0 by ss.
-                eapply M_SRC1; eauto.
-             ++ rewrite nth_error_app2 in H0 by ss.
-                assert (1 + i - List.length ths_tgt = 0)
-                  by (destruct (1 + i - List.length ths_tgt) as [|[]] in *; ss).
-                rewrite H2 in H0. inversion H0; subst.
-                lia.
+          -- enough (m_src tid0 > 1 + i) by lia. eapply M_SRC1. eauto.
+    - left.
+      match goal with
+      | [ |- paco10 _ _ _ _ _ _ _ _ _ _ _ (match ?x with
+                                          | [] => _
+                                          | t' :: ts' => _
+                                          end)] => destruct x as [| tid' ths_tgt'] eqn: E_ths_tgt
+      end.
+      { eapply app_eq_nil in E_ths_tgt. des. ss. }
+      pfold. eapply ssim_chooseL. exists tid'. unfold id_pop.
+      replace (IdSet.mem tid' (IdSet.add tid ths_src)) with true; cycle 1.
+      { symmetry. eapply IdSet.mem_1.
+        destruct ths_tgt; ss; inversion E_ths_tgt; subst.
+        - eapply IdSet.add_1; ss.
+        - eapply IdSet.add_2. eapply In_InA; eauto. rewrite THREADS. econs; ss.
+      }
+      rewrite bind_trigger. eapply ssim_fairL.
+      remember (fun i => if Nat.eqb i tid'
+                      then List.length ths_tgt' + 1
+                      else m_src i - 1) as m_src'.
+      exists m_src'. splits.
+      { ii. unfold tids_fmap. des_if; ss. subst.
+        replace (i =? tid')%nat with false by (symmetry; eapply Nat.eqb_neq; eauto).
+        des_if.
+        - assert (List.In i (IdSet.elements (IdSet.add tid ths_src))).
+          { eapply InA_In. eapply IdSet.remove_3. eapply In_InA; eauto. eapply i0. }
+          assert (i = tid \/ i <> tid) by lia.
+          destruct H0.
+          + subst. lia.
+          + assert (List.In i (IdSet.elements ths_src)).
+            { eapply InA_In. eapply IdSet.add_3; eauto. eapply In_InA; eauto. }
+            rewrite THREADS in H1. eapply In_nth_error in H1. destruct H1 as [i' H1].
+            enough (m_src i > i') by lia.
+            eapply M_SRC1; eauto.
+        - unfold le; ss. lia.
+      }
+      do 3 econs; ss. right. unfold IdSet.elt in *. eapply CIH.
+      + eapply IdSet_Permutation_remove.
+        rewrite IdSet_Permutation_add.
+        * eapply Permutation_refl' in E_ths_tgt. rewrite Permutation_app_comm in E_ths_tgt. eapply E_ths_tgt.
+        * intro H. eapply TID. eapply H.
         * ss.
-      + (* Terminate *)
-        rewrite pick_thread_nondet_terminate.
-        rewrite pick_thread_fifo_terminate.
-        destruct ths_tgt.
-        * (* ths is empty *)
-          replace (is_empty ths_src) with true.
-          2: { unfold is_empty, Raw.is_empty.
-               symmetry in THREADS.
-               eapply Permutation_nil in THREADS.
-               unfold elements, Raw.elements in THREADS.
-               rewrite THREADS.
-               ss.
-          }
-          rewrite 2 bind_ret_l.
-          rewrite interp_state_ret.
-          pfold; econs; eauto.
-        * (* ths is nonempty *)
-          replace (is_empty ths_src) with false.
-          2: { unfold is_empty, Raw.is_empty.
-               unfold elements, Raw.elements in THREADS.
-               destruct (this ths_src); eauto.
-               exfalso.
-               eapply Permutation_nil_cons; eauto.
-          }
-          destruct p as [tid' itr'].
-          rewrite bind_vis.
-          rewrite interp_state_vis.
-          rewrite bind_ret_l.
-          rewrite <- bind_trigger.
-          pfold.
-          eapply sim_chooseL.
-          exists tid'.
-          econs.
-          unfold th_pop.
-          erewrite find_1.
-          2: {
-            eapply In_MapsTo.
-            eapply Permutation_in.
-            - symmetry.
-              eapply THREADS.
-            - econs. reflexivity.
-          }
-          rewrite bind_vis.
-          rewrite interp_state_vis.
-          rewrite <- bind_trigger.
-          rewrite bind_ret_l.
-          rewrite 2 interp_state_tau.
-          eapply sim_fairL.
-          exists (fun i => match i with
-                   | inl x => if Nat.eqb x tid'
-                             then List.length ths_tgt + 1
-                             else m_src (inl x) - 1
-                   | inr x => m_src (inr x)
-                   end).
-          splits. {
-            unfold fair_update. i.
-            destruct i as [tid''|]; ss.
-            - unfold tids_fmap.
-              des_if; eauto.
-              replace (tid'' =? tid')%nat with false
-                by (symmetry; eapply Nat.eqb_neq; eauto).
-              des_if.
-              + eapply In_th_proj1 in i.
-                destruct i.
-                eapply remove_3 in H.
-                eapply elements_1 in H.
-                unfold elements, Raw.elements in H.
-                eapply setoid_in_in in H.
-                eapply Permutation_in in H.
-                2: eapply THREADS.
-                eapply In_nth_error in H.
-                destruct H as [i H].
-                enough (m_src (inl tid'') > i) by lia.
-                eapply M_SRC1.
-                eauto.
-              + unfold le, lt. ss. lia.
-            - left. eauto.
-          }
-          do 4 econs; eauto.
-          right.
-          eapply CIH1.
-          -- eapply Permutation_remove. eauto.
-          -- intros itr0 H.
-             pose proof (elements_3w ths_src).
-             eapply (Permutation_NoDupA _ _ _ THREADS) in H0.
-             inversion H0; subst.
-             eapply H3.
-             eapply SetoidList.InA_eqA; [eauto| |].
-             instantiate (1 := (tid', itr0)); ss.
-             eapply SetoidList.In_InA; [eauto|].
-             assumption.
-          -- rewrite Nat.eqb_refl. lia.
-          -- i.
-             (* tid0 can not be equal to tid', but it's easy to show [length ths_tgt + 1 > i] *)
-             des_if.
-             ++ eapply nth_error_Some' in H. lia.
-             ++ match goal with
-                | [ |- ?x - 1 > i ] => enough (x > 1 + i) by lia
-                end.
-                eapply M_SRC1.
-                eauto.
-          -- eauto.
+      + eapply IdSet.remove_1; ss.
+      + subst. replace (tid' =? tid')%nat with true by (symmetry; eapply Nat.eqb_refl). lia.
+      + subst. i. des_if.
+        * eapply nth_error_Some' in H. lia.
+        * enough (m_src tid0 > 1 + i) by lia.
+          assert (nth_error (ths_tgt ++ [tid]) (1 + i) = Some tid0) by (rewrite E_ths_tgt; ss).
+          assert (1 + i < List.length ths_tgt \/ 1 + i >= List.length ths_tgt) by lia.
+          destruct H1.
+          -- rewrite nth_error_app1 in H0 by ss. eapply M_SRC1; eauto.
+          -- rewrite nth_error_app2 in H0 by ss.
+             assert (1 + i - List.length ths_tgt = 0)
+               by (destruct (1 + i - List.length ths_tgt) as [|[]] in *; ss).
+             rewrite H2 in H0. inversion H0. subst. lia.
   Qed.
+
+  Theorem ssim_implies_gsim
+    RT R0 R1 RR p_src p_tgt sched_src sched_tgt
+    (SSIM : forall m_tgt, exists m_src, @ssim nat_wf nat_wf RT R0 R1 RR p_src m_src p_tgt m_tgt sched_src sched_tgt)
+    st (ths : @threads _Ident (sE State) RT)
+    : gsim nat_wf nat_wf RR p_src p_tgt
+        (interp_state (st, interp_sched (ths, sched_src)))
+        (interp_state (st, interp_sched (ths, sched_tgt))).
+  Proof.
+    unfold gsim. intro gm_tgt.
+
+    remember (gm_tgt ∘ inl) as m_tgt.
+    assert (M_TGT : forall i, le nat_wf (gm_tgt (inl i)) (m_tgt i)) by (subst; reflexivity).
+    specialize (SSIM m_tgt). des.
+    remember (fun (i : (sum_tid _Ident).(id)) =>
+                match i with
+                | inl i => m_src i
+                | inr i => gm_tgt (inr i)
+                end) as gm_src.
+    assert (M_SRC0 : forall i, gm_src (inl i) = m_src i) by (subst; ss).
+    assert (M_SRC1 : forall i, nat_wf.(le) (gm_tgt (inr i)) (gm_src (inr i))) by (subst; reflexivity).
+    clear Heqm_tgt Heqgm_src.
+    exists gm_src.
+ 
+    revert p_src p_tgt gm_src gm_tgt st ths m_src m_tgt sched_src sched_tgt SSIM M_TGT M_SRC0 M_SRC1.
+    ginit. gcofix CIH. i.
+
+    revert gm_src gm_tgt M_TGT M_SRC0 M_SRC1.
+    punfold SSIM. induction SSIM using ssim_ind; i.
+    - rewrite 2 interp_sched_ret, 2 interp_state_ret.
+      guclo sim_indC_spec. econs; eauto.
+    - rewrite interp_sched_tau, interp_state_tau.
+      guclo sim_indC_spec. econs. eapply IHSSIM; eauto.
+    - rewrite interp_sched_tau, interp_state_tau.
+      guclo sim_indC_spec. econs. eapply IHSSIM; eauto.
+    - pclearbot.
+      destruct (Th.find tid ths) as [t|]eqn: H0; cycle 1.
+      { rewrite 2 interp_sched_execute_None; eauto.
+        rewrite 2 interp_state_vis.
+        rewrite <- 2 bind_trigger.
+        guclo sim_indC_spec. eapply sim_indC_chooseR. ss.
+      }
+      
+      erewrite 2 interp_sched_execute_Some; eauto.
+      rewrite 2 interp_state_bind.
+      rewrite unfold_interp_thread.
+      rewrite interp_state_aux_map_event.
+
+      remember (interp_state_aux (st, interp_thread_aux (tid, t))) as itr.
+      clear Heqitr.
+
+      revert p_src p_tgt gm_src gm_tgt itr M_SRC0 M_SRC1 M_TGT.
+      gcofix CIH2; i.
+      
+      destruct_itree itr.
+      + destruct r0 as [st' lr]. rewrite map_event_ret, 2 bind_ret_l. destruct lr; ss.
+        * rewrite 2 interp_state_tau.
+          gstep. do 3 econs; eauto. gfinal. left. eapply CIH; eauto. eapply ssim_deflag, H.
+        * rewrite 2 interp_state_tau.
+          gstep. do 3 econs; eauto. gfinal. left. eapply CIH; eauto. eapply ssim_deflag, H.
+      + rewrite map_event_tau. grind.
+        gstep. do 3 econs; eauto. gfinal. left. eapply CIH2; eauto.
+      + rewrite map_event_vis, 2 bind_vis.
+        destruct e.
+        * rewrite <- 2 bind_trigger.
+          gstep. eapply sim_chooseR. i. eapply sim_chooseL. exists x. econs; eauto. gfinal. left. eapply CIH2; eauto.
+        * rewrite <- 2 bind_trigger.
+          gstep. eapply sim_fairR. intros gm_tgt0 FAIR. eapply sim_fairL.
+          remember (fun i => match i with
+                          | inl i => gm_src (inl i)
+                          | inr i => gm_tgt0 (inr i)
+                          end) as gm_src0.
+          exists gm_src0. splits.
+          { subst. intros []; ss.
+            - reflexivity.
+            - specialize (FAIR (inr i)). specialize (M_SRC1 i). unfold le in *; ss. destruct (m i); lia.
+          }
+          econs; eauto. gfinal. left. eapply CIH2.
+          -- subst; eauto.
+          -- subst; reflexivity.
+          -- i. specialize (FAIR (inl i)). specialize (M_TGT i). unfold le in *; ss. lia.
+        * gstep. econs. i. subst. gfinal. left. eapply CIH2; eauto.
+        * rewrite <- 2 bind_trigger. gstep. eapply sim_ub.
+    - rewrite 2 interp_sched_vis, 2 interp_state_vis.
+      gstep. econs. i. subst.
+      rewrite 2 interp_state_tau.
+      gstep. do 5 econs; eauto. pclearbot. gfinal. left. eapply CIH; ss. eapply ssim_deflag. eapply H.
+    - des. rewrite interp_sched_vis, interp_state_vis, <- bind_trigger.
+      guclo sim_indC_spec. econs. eexists.
+      rewrite interp_state_tau.
+      do 2 (guclo sim_indC_spec; econs). eapply H0; eauto.
+    - rewrite interp_sched_vis, interp_state_vis, <- bind_trigger.
+      guclo sim_indC_spec. econs. i.
+      rewrite interp_state_tau.
+      do 2 (guclo sim_indC_spec; econs). eapply H0; eauto.
+    - des. rewrite interp_sched_vis, interp_state_vis, <- bind_trigger.
+      guclo sim_indC_spec. econs.
+      remember (fun (i : (sum_tid _Ident).(id)) =>
+                  match i with
+                  | inl i => m_src0 i
+                  | inr i => gm_tgt (inr i)
+                  end) as gm_src0.
+      exists gm_src0. splits.
+      { subst. intros []; ss. rewrite M_SRC0. eapply FAIR. }
+      rewrite interp_state_tau.
+      do 2 (guclo sim_indC_spec; econs). eapply H1; subst; eauto. reflexivity.
+    - rewrite interp_sched_vis, interp_state_vis, <- bind_trigger.
+      guclo sim_indC_spec. econs. intros gm_tgt0 FAIR.
+      rewrite interp_state_tau.
+      do 2 (guclo sim_indC_spec; econs). eapply H0. instantiate (1 := fun i => gm_tgt0 (inl i)).
+      + ii. specialize (FAIR (inl i)). specialize (M_TGT i). unfold le in *; ss. destruct (f_tgt i); lia.
+      + reflexivity.
+      + eauto.
+      + i. specialize (FAIR (inr i)). specialize (M_SRC1 i). unfold le in *; ss. lia.
+    - rewrite interp_sched_vis, interp_state_vis, <- bind_trigger. ss.
+      gstep. eapply sim_ub.
+    - gstep. econs; eauto. pclearbot. gfinal. left. eapply CIH; eauto.
+  Qed.
+
+  Check ssim_nondet_fifo.
+  Check ssim_implies_gsim.
+
+  Definition key_set {elt} : Th.t elt -> IdSet.t.
+  Proof.
+    intros [l SORTED]. unfold Raw.t in *.
+    set (l' := List.map fst l).
+    econs. instantiate (1 := l').
+    unfold Raw.PX.ltk in *.
+
+    assert (Sorted (fun x y => x < y) l').
+    { induction SORTED.
+      - subst l'. ss.
+      - subst l'. ss. econs 2; ss.
+        inv H; ss. econs; ss.
+    }
+    
+    eapply IdSet.MSet.Raw.isok_iff. ss.
+  Defined.
+
+  Theorem sched_sim p_src p_tgt tid st (ths : @threads _Ident (sE State) R) (TID : ~ IdSet.In tid (key_set ths))
+    : gsim nat_wf nat_wf eq p_src p_tgt
+        (interp_state (st, interp_sched (ths, schedule_nondet _ (tid, key_set ths))))
+        (interp_state (st, interp_sched (ths, schedule_fifo _ (tid, IdSet.elements (key_set ths))))).
+  Proof. eapply ssim_implies_gsim. eapply ssim_nondet_fifo; ss. Qed.
 
 End SIM.
